Tensor product lore

DeBruijnSSA/BinSyntax/Rewrite/Categorical.lean
@@ -13,23 +13,70 @@ theorem Wf.ret {tyIn tyOut : Ty α} {rest: Ctx α ε} {targets : LCtx α}
 
 def InS.ret {tyIn tyOut : Ty α} {rest: Ctx α ε} {targets : LCtx α}
   (t : Term.InS φ (⟨tyIn, ⊥⟩::rest) ⟨tyOut, ⊥⟩)
-  : InS φ (⟨tyIn, ⊥⟩::rest) (tyOut::targets) := ⟨Region.ret t, Wf.ret t.prop⟩
+  : InS φ (⟨tyIn, ⊥⟩::rest) (tyOut::targets) := InS.br 0 t ⟨by simp, le_refl _⟩
+
+theorem InS.ret_eq {tyIn tyOut : Ty α} {rest: Ctx α ε} {targets : LCtx α}
+  (t : Term.InS φ (⟨tyIn, ⊥⟩::rest) ⟨tyOut, ⊥⟩)
+  : InS.ret (targets := targets) t = ⟨Region.ret t, Wf.ret t.prop⟩ := rfl
+
+theorem InS.vwk_ret {tyIn tyOut : Ty α} {rest: Ctx α ε} {targets : LCtx α}
+  (ρ : Ctx.InS (⟨tyIn, ⊥⟩::rest') _)
+  (t : Term.InS φ (⟨tyIn, ⊥⟩::rest) ⟨tyOut, ⊥⟩)
+  : (InS.ret (targets := targets) t).vwk ρ = InS.ret (t.wk ρ) := rfl
 
 abbrev Eqv.ret {tyIn tyOut : Ty α} {rest: Ctx α ε} {targets : LCtx α}
   (t : Term.InS φ (⟨tyIn, ⊥⟩::rest) ⟨tyOut, ⊥⟩)
   : Eqv φ (⟨tyIn, ⊥⟩::rest) (tyOut::targets) := ⟦InS.ret t⟧
 
+theorem Eqv.vwk_ret {tyIn tyOut : Ty α} {rest: Ctx α ε} {targets : LCtx α}
+  (ρ : Ctx.InS (⟨tyIn, ⊥⟩::rest') _)
+  (t : Term.InS φ (⟨tyIn, ⊥⟩::rest) ⟨tyOut, ⊥⟩)
+  : (Eqv.ret (targets := targets) t).vwk ρ = Eqv.ret (t.wk ρ) := rfl
+
 theorem Wf.nil {ty : Ty α} {rest: Ctx α ε} {targets : LCtx α}
   : Region.nil.Wf (φ := φ) (⟨ty, ⊥⟩::rest) (ty::targets) := Wf.ret (by simp)
 
 def InS.nil {ty : Ty α} {rest: Ctx α ε} {targets : LCtx α}
-  : InS φ (⟨ty, ⊥⟩::rest) (ty::targets)  := ⟨Region.nil, Wf.nil⟩
+  : InS φ (⟨ty, ⊥⟩::rest) (ty::targets)  := InS.ret (Term.InS.var 0 (by simp))
+
+theorem InS.nil_eq {ty : Ty α} {rest: Ctx α ε} {targets : LCtx α}
+  : InS.nil (φ := φ) (ty := ty) (rest := rest) (targets := targets) = ⟨Region.nil, Wf.nil⟩ := rfl
+
+@[simp]
+theorem InS.nil_vwk_lift (ρ : Ctx.InS rest _)
+  : (InS.nil (φ := φ) (ty := ty) (rest := rest') (targets := targets)).vwk (ρ.lift h) = InS.nil
+  := rfl
+
+@[simp]
+theorem InS.nil_vwk1
+  : (InS.nil (φ := φ) (ty := ty) (rest := rest) (targets := targets)).vwk1 (right := right)
+  = InS.nil := rfl
 
 -- theorem InS.coe_nil {ty : Ty α} {rest: Ctx α ε} {targets : LCtx α}
 --   : (InS.nil (ty := ty) (rest := rest) (targets := targets) : Region φ) = Region.nil := rfl
 
 abbrev Eqv.nil {ty : Ty α} {rest: Ctx α ε} {targets : LCtx α}
   : Eqv φ (⟨ty, ⊥⟩::rest) (ty::targets) := ⟦InS.nil⟧
+
+@[simp]
+theorem Eqv.nil_vwk_lift (ρ : Ctx.InS rest _)
+  : (Eqv.nil (φ := φ) (ty := ty) (rest := rest') (targets := targets)).vwk (ρ.lift h) = Eqv.nil
+  := rfl
+
+@[simp]
+theorem Eqv.nil_vwk_liftn₂ (ρ : Ctx.InS rest _)
+  : (Eqv.nil (φ := φ) (ty := ty) (rest := (head'::rest')) (targets := targets)).vwk (ρ.liftn₂ h h')
+  = Eqv.nil
+  := rfl
+
+theorem Eqv.nil_vwk1 {Γ : Ctx α ε} {L : LCtx α}
+  : (Eqv.nil (φ := φ) (ty := ty) (rest := Γ) (targets := L)).vwk1 (inserted := inserted)
+  = Eqv.nil := rfl
+
+theorem Eqv.let1_0_nil
+  : Eqv.let1 (Term.InS.var 0 ⟨by simp, le_refl _⟩) Eqv.nil
+  = Eqv.nil (φ := φ) (ty := ty) (rest := rest) (targets := targets)
+  := by rw [let1_beta]; rfl
 
 def Wf.lsubst0 {Γ : Ctx α ε} {L : LCtx α} {r : Region φ} (hr : r.Wf (⟨A, ⊥⟩::Γ) L)
   : r.lsubst0.Wf Γ (A::L) L
@@ -59,9 +106,24 @@ theorem InS.alpha0_congr {A B : Ty α} {Γ : Ctx α ε} {L : LCtx α} {r r' : In
   (h : r ≈ r') : InS.alpha0 r ≈ InS.alpha0 r'
   := sorry
 
+theorem InS.vlift_alpha0 {A B : Ty α} {Γ : Ctx α ε} {L : LCtx α} (r : InS φ (⟨A, ⊥⟩::Γ) (B::L))
+  : (InS.alpha0 r).vlift = InS.alpha0 (r.vwk1 (right := X)) := by
+  simp only [Subst.InS.vlift, Set.mem_setOf_eq, alpha0, vlift_alpha]
+  rfl
+
 def Eqv.alpha0 {A B : Ty α} {Γ : Ctx α ε} {L : LCtx α} (r : Eqv φ (⟨A, ⊥⟩::Γ) (B::L))
   : Subst.Eqv φ Γ (A::L) (B::L)
   := Quot.liftOn r (λr => ⟦InS.alpha0 r⟧) (λ_ _ h => Quotient.sound $ InS.alpha0_congr h)
+
+@[simp]
+theorem Eqv.alpha0_quot {A B : Ty α} {Γ : Ctx α ε} {L : LCtx α} (r : InS φ (⟨A, ⊥⟩::Γ) (B::L))
+  : Eqv.alpha0 ⟦r⟧ = ⟦InS.alpha0 r⟧ := rfl
+
+theorem Eqv.vlift_alpha0 {A B : Ty α} {Γ : Ctx α ε} {L : LCtx α} (r : Eqv φ (⟨A, ⊥⟩::Γ) (B::L))
+  : (Eqv.alpha0 r).vlift = Eqv.alpha0 (r.vwk1 (inserted := X)) := by
+  induction r using Quotient.inductionOn;
+  rw [alpha0_quot, Subst.Eqv.vlift_quot, InS.vlift_alpha0]
+  rfl
 
 def InS.seq {A B C : Ty α} {Γ : Ctx α ε} {L : LCtx α}
   (left : InS φ (⟨A, ⊥⟩::Γ) (B::L)) (right : InS φ (⟨B, ⊥⟩::Γ) (C::L)) : InS φ (⟨A, ⊥⟩::Γ) (C::L)
@@ -89,13 +151,13 @@ theorem InS.append_mk {A B C : Ty α} {Γ : Ctx α ε} {L : LCtx α}
 theorem InS.append_nil {A B : Ty α} {Γ : Ctx α ε} {L : LCtx α}
   {l : InS φ (⟨A, ⊥⟩::Γ) (B::L)}
   : (l ++ InS.nil (φ := φ) (ty := B) (rest := Γ) (targets := L)) = l := by
-  cases l; simp [InS.nil, append_mk, Region.append_nil]
+  cases l; simp [nil_eq, append_mk, Region.append_nil]
 
 @[simp]
 theorem InS.nil_append {A B : Ty α} {Γ : Ctx α ε} {L : LCtx α}
   {l : InS φ (⟨A, ⊥⟩::Γ) (B::L)}
   : (InS.nil (φ := φ) (ty := A) (rest := Γ) (targets := L) ++ l) = l := by
-  cases l; simp [InS.nil, append_mk, Region.nil_append]
+  cases l; simp [nil_eq, append_mk, Region.nil_append]
 
 theorem InS.append_assoc {A B C D : Ty α} {Γ : Ctx α ε} {L : LCtx α}
   (left : InS φ (⟨A, ⊥⟩::Γ) (B::L))
@@ -104,6 +166,14 @@ theorem InS.append_assoc {A B C D : Ty α} {Γ : Ctx α ε} {L : LCtx α}
   : (left ++ middle) ++ right = left ++ (middle ++ right) := by
   cases left; cases middle; cases right;
   simp [append_mk, Region.append_assoc]
+
+-- theorem InS.let1_seq {Γ : Ctx α ε} {L : LCtx α}
+--   (a : Term.InS φ (⟨A, ⊥⟩::Γ) ⟨X, e⟩)
+--   (r : InS φ (⟨X, ⊥⟩::⟨A, ⊥⟩::Γ) (B::L)) (s : InS φ (⟨B, ⊥⟩::Γ) (C::L))
+--   : (let1 a r) ++ s = let1 a (r ++ (s.vwk1 (right := ⟨X, ⊥⟩))) := by
+--   induction r using Quotient.inductionOn;
+--   induction s using Quotient.inductionOn;
+--   sorry
 
 def Eqv.seq {A B C : Ty α} {Γ : Ctx α ε} {L : LCtx α}
   (left : Eqv φ (⟨A, ⊥⟩::Γ) (B::L)) (right : Eqv φ (⟨B, ⊥⟩::Γ) (C::L)) : Eqv φ (⟨A, ⊥⟩::Γ) (C::L)
@@ -159,6 +229,80 @@ theorem Eqv.seq_assoc {A B C D : Ty α} {Γ : Ctx α ε} {L : LCtx α}
   induction right using Quotient.inductionOn;
   simp [InS.append_assoc]
 
+theorem Eqv.ret_seq {A B C : Ty α} {Γ : Ctx α ε} {L : LCtx α}
+  (a : Term.InS φ (⟨A, ⊥⟩::Γ) ⟨B, ⊥⟩)
+  (r : Eqv φ (⟨B, ⊥⟩::Γ) (C::L))
+  : (Eqv.ret a) ;; r = r.vwk1.vsubst a.subst0 := by
+  induction r using Quotient.inductionOn;
+  simp only [ret, seq_def, vwk1_quot, alpha0_quot, lsubst_quot, vsubst_quot]
+  rfl
+
+theorem Eqv.ret_seq_let {A B C : Ty α} {Γ : Ctx α ε} {L : LCtx α}
+  (a : Term.InS φ (⟨A, ⊥⟩::Γ) ⟨B, ⊥⟩)
+  (r : Eqv φ (⟨B, ⊥⟩::Γ) (C::L))
+  : (Eqv.ret a) ;; r = let1 a r.vwk1 := by rw [ret_seq, let1_beta]
+
+theorem Eqv.let1_seq {Γ : Ctx α ε} {L : LCtx α}
+  (a : Term.InS φ (⟨A, ⊥⟩::Γ) ⟨X, e⟩)
+  (r : Eqv φ (⟨X, ⊥⟩::⟨A, ⊥⟩::Γ) (B::L)) (s : Eqv φ (⟨B, ⊥⟩::Γ) (C::L))
+  : (Eqv.let1 a r) ;; s = Eqv.let1 a (r ;; s.vwk1) := by
+  simp only [seq_def, lsubst_let1, vlift_alpha0]
+
+theorem Eqv.let2_seq {Γ : Ctx α ε} {L : LCtx α}
+  (a : Term.InS φ (⟨A, ⊥⟩::Γ) ⟨X.prod Y, e⟩)
+  (r : Eqv φ (⟨Y, ⊥⟩::⟨X, ⊥⟩::⟨A, ⊥⟩::Γ) (C::L)) (s : Eqv φ (⟨C, ⊥⟩::Γ) (D::L))
+  : (Eqv.let2 a r) ;; s = Eqv.let2 a (r ;; s.vwk1.vwk1) := by
+  simp only [seq_def, lsubst_let2, Subst.Eqv.vliftn₂_eq_vlift_vlift, vlift_alpha0]
+
+theorem Eqv.case_seq {Γ : Ctx α ε} {L : LCtx α}
+  (a : Term.InS φ (⟨A, ⊥⟩::Γ) ⟨X.coprod Y, e⟩)
+  (r : Eqv φ (⟨X, ⊥⟩::⟨A, ⊥⟩::Γ) (B::L)) (s : Eqv φ (⟨Y, ⊥⟩::⟨A, ⊥⟩::Γ) (B::L))
+  (t : Eqv φ (⟨B, ⊥⟩::Γ) (C::L))
+  : (Eqv.case a r s) ;; t = Eqv.case a (r ;; t.vwk1) (s ;; t.vwk1) := by
+  simp only [seq_def, lsubst_case, vlift_alpha0]
+
+theorem Eqv.vwk_lift_seq {A B C : Ty α} {Γ Δ : Ctx α ε} {L : LCtx α}
+  (ρ : Ctx.InS Γ Δ)
+  (left : Eqv φ (⟨A, ⊥⟩::Δ) (B::L))
+  (right : Eqv φ (⟨B, ⊥⟩::Δ) (C::L))
+  : (left ;; right).vwk (ρ.lift (le_refl _))
+  = left.vwk (ρ.lift (le_refl _)) ;; right.vwk (ρ.lift (le_refl _)) := by
+  induction left using Quotient.inductionOn;
+  induction right using Quotient.inductionOn;
+  sorry
+
+theorem Eqv.vwk_liftn₂_seq {A B C : Ty α} {Γ Δ : Ctx α ε} {L : LCtx α}
+  (ρ : Ctx.InS Γ Δ)
+  (left : Eqv φ (⟨A, ⊥⟩::X::Δ) (B::L))
+  (right : Eqv φ (⟨B, ⊥⟩::X::Δ) (C::L))
+  : (left ;; right).vwk (ρ.liftn₂ (le_refl _) (le_refl _))
+  = left.vwk (ρ.liftn₂ (le_refl _) (le_refl _)) ;; right.vwk (ρ.liftn₂ (le_refl _) (le_refl _))
+  := by simp only [<-Ctx.InS.lift_lift, vwk_lift_seq]
+
+theorem Eqv.vwk1_seq {A B C : Ty α} {Γ : Ctx α ε} {L : LCtx α}
+  (left : Eqv φ (⟨A, ⊥⟩::Γ) (B::L))
+  (right : Eqv φ (⟨B, ⊥⟩::Γ) (C::L))
+  : (left ;; right).vwk1 (inserted := inserted)
+  = left.vwk1 ;; right.vwk1 := vwk_lift_seq ⟨Nat.succ, (by simp)⟩ left right
+
+theorem Eqv.vsubst_lift_seq {A B C : Ty α} {Γ Δ : Ctx α ε} {L : LCtx α}
+  (σ : Term.Subst.InS φ Γ Δ)
+  (left : Eqv φ (⟨A, ⊥⟩::Δ) (B::L))
+  (right : Eqv φ (⟨B, ⊥⟩::Δ) (C::L))
+  : (left ;; right).vsubst (σ.lift (le_refl _))
+  = left.vsubst (σ.lift (le_refl _)) ;; right.vsubst (σ.lift (le_refl _)) := by
+  induction left using Quotient.inductionOn;
+  induction right using Quotient.inductionOn;
+  sorry
+
+theorem Eqv.vsubst_liftn₂_seq {A B C : Ty α} {Γ Δ : Ctx α ε} {L : LCtx α}
+  (σ : Term.Subst.InS φ Γ Δ)
+  (left : Eqv φ (⟨A, ⊥⟩::X::Δ) (B::L))
+  (right : Eqv φ (⟨B, ⊥⟩::X::Δ) (C::L))
+  : (left ;; right).vsubst (σ.liftn₂ (le_refl _) (le_refl _))
+  = left.vsubst (σ.liftn₂ (le_refl _) (le_refl _)) ;; right.vsubst (σ.liftn₂ (le_refl _) (le_refl _))
+  := by simp only [<-Term.Subst.InS.lift_lift, vsubst_lift_seq]
+
 open Term.InS
 
 def Eqv.rtimes {tyIn tyOut : Ty α} {Γ : Ctx α ε} {L : LCtx α}
@@ -173,13 +317,45 @@ def Eqv.swap {left right : Ty α} {Γ : Ctx α ε} {L : LCtx α}
   := Eqv.let2 (var 0 Ctx.Var.shead) $
   ret (pair (var 0 (by simp)) (var 1 (by simp)))
 
+theorem Eqv.repack {left right : Ty α} {rest : Ctx α ε} {targets : LCtx α}
+  : Eqv.let2 (Term.InS.var 0 ⟨by simp, le_refl _⟩)
+    (Eqv.ret (Term.InS.pair (Term.InS.var 1 (by simp)) (Term.InS.var 0 (by simp))))
+  = Eqv.nil (φ := φ) (ty := left.prod right) (rest := rest) (targets := targets) := by
+  rw [<-let1_0_nil, <-let2_eta, let1_beta]
+  rfl
+
 theorem Eqv.swap_swap {left right : Ty α}
   : Eqv.swap ;; Eqv.swap
   = (Eqv.nil (φ := φ) (ty := left.prod right) (rest := rest) (targets := targets)) := by
-  rw [Eqv.seq_def, swap, vwk1, swap]
-  sorry
+  simp only [
+    swap, let2_seq, vwk1, vwk_let2, wk_var, wk_pair, Nat.liftWk, vwk_ret, Ctx.InS.liftn₂,
+    Nat.liftnWk, Nat.one_lt_ofNat, Nat.ofNat_pos, ↓reduceIte, ret_seq, vsubst_let2,
+    subst_pair, subst_var, Term.Subst.InS.get_0_subst0, let2_pair, let1_beta, vsubst_vsubst
+  ]
+  apply Eqv.repack
 
 infixl:70 " ⋊ "  => Eqv.rtimes
+
+theorem Eqv.rtimes_nil {ty : Ty α} {Γ : Ctx α ε} {L : LCtx α}
+  (tyLeft : Ty α)
+  : tyLeft ⋊ Eqv.nil = (Eqv.nil (φ := φ) (ty := tyLeft.prod ty) (rest := Γ) (targets := L)) := by
+  simp only [rtimes, nil_vwk1, nil_seq, repack]
+
+theorem Eqv.rtimes_seq {A B C : Ty α} {Γ : Ctx α ε} {L : LCtx α}
+  (tyLeft : Ty α) (r : Eqv φ (⟨A, ⊥⟩::Γ) (B::L)) (s : Eqv φ (⟨B, ⊥⟩::Γ) (C::L))
+  : tyLeft ⋊ (r ;; s) = (tyLeft ⋊ r) ;; (tyLeft ⋊ s) := by
+  apply Eq.symm
+  rw [rtimes, rtimes, let2_seq, seq_assoc, ret_seq]
+  simp only [
+    vwk1, vwk_let2, wk_var, Nat.liftWk, vsubst_let2, vwk_vwk, Ctx.InS.liftn₂_comp_liftn₂,
+    subst_pair, subst_var, Term.Subst.InS.get_0_subst0, let2_pair, let1_beta,
+    vsubst_vsubst
+  ]
+  apply congrArg
+  rw [vwk1_seq, vwk1_seq, seq_assoc]
+  congr 1
+  . simp [vwk1, vwk_vwk]
+  . sorry
 
 def Eqv.ltimes {tyIn tyOut : Ty α} {Γ : Ctx α ε} {L : LCtx α}
   (r : Eqv φ (⟨tyIn, ⊥⟩::Γ) (tyOut::L)) (tyRight : Ty α)
@@ -203,3 +379,17 @@ theorem Eqv.swap_ltimes_swap {Γ : Ctx α ε} {L : LCtx α}
   : Eqv.swap ;; r ⋉ C ;; Eqv.swap = C ⋊ r
   := by rw [
     ltimes, seq_assoc, seq_assoc, swap_swap, seq_assoc, seq_nil, <-seq_assoc, swap_swap, nil_seq]
+
+theorem Eqv.ltimes_nil {ty : Ty α} {Γ : Ctx α ε} {L : LCtx α}
+  : Eqv.nil ⋉ tyRight = (Eqv.nil (φ := φ) (ty := ty.prod tyRight) (rest := Γ) (targets := L))
+  := by rw [<-swap_rtimes_swap, rtimes_nil, seq_nil, swap_swap]
+
+theorem Eqv.ltimes_seq {A B C : Ty α} {Γ : Ctx α ε} {L : LCtx α}
+  (r : Eqv φ (⟨A, ⊥⟩::Γ) (B::L)) (s : Eqv φ (⟨B, ⊥⟩::Γ) (C::L))
+  : (r ;; s) ⋉ tyRight = (r ⋉ tyRight) ;; (s ⋉ tyRight) := by
+  simp only [<-swap_rtimes_swap, rtimes_seq, seq_assoc]
+  rw [<-seq_assoc swap swap, swap_swap, nil_seq]
+
+end Region
+
+end BinSyntax
